# Commutative rings

<pre class="Agda"><a id="30" class="Symbol">{-#</a> <a id="34" class="Keyword">OPTIONS</a> <a id="42" class="Pragma">--without-K</a> <a id="54" class="Pragma">--exact-split</a> <a id="68" class="Symbol">#-}</a>

<a id="73" class="Keyword">module</a> <a id="80" href="ring-theory.commutative-rings.html" class="Module">ring-theory.commutative-rings</a> <a id="110" class="Keyword">where</a>

<a id="117" class="Keyword">open</a> <a id="122" class="Keyword">import</a> <a id="129" href="foundation.dependent-pair-types.html" class="Module">foundation.dependent-pair-types</a> <a id="161" class="Keyword">using</a> <a id="167" class="Symbol">(</a><a id="168" href="foundation-core.dependent-pair-types.html#502" class="Record">Σ</a><a id="169" class="Symbol">;</a> <a id="171" href="foundation-core.dependent-pair-types.html#575" class="InductiveConstructor">pair</a><a id="175" class="Symbol">;</a> <a id="177" href="foundation-core.dependent-pair-types.html#592" class="Field">pr1</a><a id="180" class="Symbol">;</a> <a id="182" href="foundation-core.dependent-pair-types.html#604" class="Field">pr2</a><a id="185" class="Symbol">)</a>
<a id="187" class="Keyword">open</a> <a id="192" class="Keyword">import</a> <a id="199" href="foundation.identity-types.html" class="Module">foundation.identity-types</a> <a id="225" class="Keyword">using</a> <a id="231" class="Symbol">(</a><a id="232" href="foundation-core.identity-types.html#641" class="Datatype">Id</a><a id="234" class="Symbol">)</a>
<a id="236" class="Keyword">open</a> <a id="241" class="Keyword">import</a> <a id="248" href="foundation.propositions.html" class="Module">foundation.propositions</a> <a id="272" class="Keyword">using</a> <a id="278" class="Symbol">(</a><a id="279" href="foundation-core.propositions.html#1246" class="Function">is-prop</a><a id="286" class="Symbol">;</a> <a id="288" href="foundation.propositions.html#1492" class="Function">is-prop-Π</a><a id="297" class="Symbol">)</a>
<a id="299" class="Keyword">open</a> <a id="304" class="Keyword">import</a> <a id="311" href="foundation.universe-levels.html" class="Module">foundation.universe-levels</a> <a id="338" class="Keyword">using</a> <a id="344" class="Symbol">(</a><a id="345" href="Agda.Primitive.html#597" class="Postulate">Level</a><a id="350" class="Symbol">;</a> <a id="352" href="foundation-core.universe-levels.html#222" class="Primitive">UU</a><a id="354" class="Symbol">;</a> <a id="356" href="Agda.Primitive.html#780" class="Primitive">lsuc</a><a id="360" class="Symbol">)</a>

<a id="363" class="Keyword">open</a> <a id="368" class="Keyword">import</a> <a id="375" href="ring-theory.rings.html" class="Module">ring-theory.rings</a> <a id="393" class="Keyword">using</a>
  <a id="401" class="Symbol">(</a> <a id="403" href="ring-theory.rings.html#1734" class="Function">Ring</a><a id="407" class="Symbol">;</a> <a id="409" href="ring-theory.rings.html#2030" class="Function">type-Ring</a><a id="418" class="Symbol">;</a> <a id="420" href="ring-theory.rings.html#4490" class="Function">mul-Ring</a><a id="428" class="Symbol">;</a> <a id="430" href="ring-theory.rings.html#2111" class="Function">is-set-type-Ring</a><a id="446" class="Symbol">)</a>
</pre>
## Idea

A ring `R` is said to be commutative if its multiplicative operation is commutative, i.e., if `xy = yx` for all `x, y ∈ R`.

## Definition

<pre class="Agda"><a id="is-commutative-Ring"></a><a id="610" href="ring-theory.commutative-rings.html#610" class="Function">is-commutative-Ring</a> <a id="630" class="Symbol">:</a>
  <a id="634" class="Symbol">{</a> <a id="636" href="ring-theory.commutative-rings.html#636" class="Bound">l</a> <a id="638" class="Symbol">:</a> <a id="640" href="Agda.Primitive.html#597" class="Postulate">Level</a><a id="645" class="Symbol">}</a> <a id="647" class="Symbol">→</a> <a id="649" href="ring-theory.rings.html#1734" class="Function">Ring</a> <a id="654" href="ring-theory.commutative-rings.html#636" class="Bound">l</a> <a id="656" class="Symbol">→</a> <a id="658" href="foundation-core.universe-levels.html#222" class="Primitive">UU</a> <a id="661" href="ring-theory.commutative-rings.html#636" class="Bound">l</a>
<a id="663" href="ring-theory.commutative-rings.html#610" class="Function">is-commutative-Ring</a> <a id="683" href="ring-theory.commutative-rings.html#683" class="Bound">R</a> <a id="685" class="Symbol">=</a>
  <a id="689" class="Symbol">(</a><a id="690" href="ring-theory.commutative-rings.html#690" class="Bound">x</a> <a id="692" href="ring-theory.commutative-rings.html#692" class="Bound">y</a> <a id="694" class="Symbol">:</a> <a id="696" href="ring-theory.rings.html#2030" class="Function">type-Ring</a> <a id="706" href="ring-theory.commutative-rings.html#683" class="Bound">R</a><a id="707" class="Symbol">)</a> <a id="709" class="Symbol">→</a> <a id="711" href="foundation-core.identity-types.html#641" class="Datatype">Id</a> <a id="714" class="Symbol">(</a><a id="715" href="ring-theory.rings.html#4490" class="Function">mul-Ring</a> <a id="724" href="ring-theory.commutative-rings.html#683" class="Bound">R</a> <a id="726" href="ring-theory.commutative-rings.html#690" class="Bound">x</a> <a id="728" href="ring-theory.commutative-rings.html#692" class="Bound">y</a><a id="729" class="Symbol">)</a> <a id="731" class="Symbol">(</a><a id="732" href="ring-theory.rings.html#4490" class="Function">mul-Ring</a> <a id="741" href="ring-theory.commutative-rings.html#683" class="Bound">R</a> <a id="743" href="ring-theory.commutative-rings.html#692" class="Bound">y</a> <a id="745" href="ring-theory.commutative-rings.html#690" class="Bound">x</a><a id="746" class="Symbol">)</a>

<a id="is-prop-is-commutative-Ring"></a><a id="749" href="ring-theory.commutative-rings.html#749" class="Function">is-prop-is-commutative-Ring</a> <a id="777" class="Symbol">:</a>
  <a id="781" class="Symbol">{</a> <a id="783" href="ring-theory.commutative-rings.html#783" class="Bound">l</a> <a id="785" class="Symbol">:</a> <a id="787" href="Agda.Primitive.html#597" class="Postulate">Level</a><a id="792" class="Symbol">}</a> <a id="794" class="Symbol">(</a><a id="795" href="ring-theory.commutative-rings.html#795" class="Bound">R</a> <a id="797" class="Symbol">:</a> <a id="799" href="ring-theory.rings.html#1734" class="Function">Ring</a> <a id="804" href="ring-theory.commutative-rings.html#783" class="Bound">l</a><a id="805" class="Symbol">)</a> <a id="807" class="Symbol">→</a> <a id="809" href="foundation-core.propositions.html#1246" class="Function">is-prop</a> <a id="817" class="Symbol">(</a><a id="818" href="ring-theory.commutative-rings.html#610" class="Function">is-commutative-Ring</a> <a id="838" href="ring-theory.commutative-rings.html#795" class="Bound">R</a><a id="839" class="Symbol">)</a>
<a id="841" href="ring-theory.commutative-rings.html#749" class="Function">is-prop-is-commutative-Ring</a> <a id="869" href="ring-theory.commutative-rings.html#869" class="Bound">R</a> <a id="871" class="Symbol">=</a>
  <a id="875" href="foundation.propositions.html#1492" class="Function">is-prop-Π</a>
    <a id="889" class="Symbol">(</a> <a id="891" class="Symbol">λ</a> <a id="893" href="ring-theory.commutative-rings.html#893" class="Bound">x</a> <a id="895" class="Symbol">→</a>
      <a id="903" href="foundation.propositions.html#1492" class="Function">is-prop-Π</a>
      <a id="919" class="Symbol">(</a> <a id="921" class="Symbol">λ</a> <a id="923" href="ring-theory.commutative-rings.html#923" class="Bound">y</a> <a id="925" class="Symbol">→</a>
        <a id="935" href="ring-theory.rings.html#2111" class="Function">is-set-type-Ring</a> <a id="952" href="ring-theory.commutative-rings.html#869" class="Bound">R</a> <a id="954" class="Symbol">(</a><a id="955" href="ring-theory.rings.html#4490" class="Function">mul-Ring</a> <a id="964" href="ring-theory.commutative-rings.html#869" class="Bound">R</a> <a id="966" href="ring-theory.commutative-rings.html#893" class="Bound">x</a> <a id="968" href="ring-theory.commutative-rings.html#923" class="Bound">y</a><a id="969" class="Symbol">)</a> <a id="971" class="Symbol">(</a><a id="972" href="ring-theory.rings.html#4490" class="Function">mul-Ring</a> <a id="981" href="ring-theory.commutative-rings.html#869" class="Bound">R</a> <a id="983" href="ring-theory.commutative-rings.html#923" class="Bound">y</a> <a id="985" href="ring-theory.commutative-rings.html#893" class="Bound">x</a><a id="986" class="Symbol">)))</a>

<a id="Comm-Ring"></a><a id="991" href="ring-theory.commutative-rings.html#991" class="Function">Comm-Ring</a> <a id="1001" class="Symbol">:</a>
  <a id="1005" class="Symbol">(</a> <a id="1007" href="ring-theory.commutative-rings.html#1007" class="Bound">l</a> <a id="1009" class="Symbol">:</a> <a id="1011" href="Agda.Primitive.html#597" class="Postulate">Level</a><a id="1016" class="Symbol">)</a> <a id="1018" class="Symbol">→</a> <a id="1020" href="foundation-core.universe-levels.html#222" class="Primitive">UU</a> <a id="1023" class="Symbol">(</a><a id="1024" href="Agda.Primitive.html#780" class="Primitive">lsuc</a> <a id="1029" href="ring-theory.commutative-rings.html#1007" class="Bound">l</a><a id="1030" class="Symbol">)</a>
<a id="1032" href="ring-theory.commutative-rings.html#991" class="Function">Comm-Ring</a> <a id="1042" href="ring-theory.commutative-rings.html#1042" class="Bound">l</a> <a id="1044" class="Symbol">=</a> <a id="1046" href="foundation-core.dependent-pair-types.html#502" class="Record">Σ</a> <a id="1048" class="Symbol">(</a><a id="1049" href="ring-theory.rings.html#1734" class="Function">Ring</a> <a id="1054" href="ring-theory.commutative-rings.html#1042" class="Bound">l</a><a id="1055" class="Symbol">)</a> <a id="1057" href="ring-theory.commutative-rings.html#610" class="Function">is-commutative-Ring</a>

<a id="ring-Comm-Ring"></a><a id="1078" href="ring-theory.commutative-rings.html#1078" class="Function">ring-Comm-Ring</a> <a id="1093" class="Symbol">:</a>
  <a id="1097" class="Symbol">{</a> <a id="1099" href="ring-theory.commutative-rings.html#1099" class="Bound">l</a> <a id="1101" class="Symbol">:</a> <a id="1103" href="Agda.Primitive.html#597" class="Postulate">Level</a><a id="1108" class="Symbol">}</a> <a id="1110" class="Symbol">→</a> <a id="1112" href="ring-theory.commutative-rings.html#991" class="Function">Comm-Ring</a> <a id="1122" href="ring-theory.commutative-rings.html#1099" class="Bound">l</a> <a id="1124" class="Symbol">→</a> <a id="1126" href="ring-theory.rings.html#1734" class="Function">Ring</a> <a id="1131" href="ring-theory.commutative-rings.html#1099" class="Bound">l</a>
<a id="1133" href="ring-theory.commutative-rings.html#1078" class="Function">ring-Comm-Ring</a> <a id="1148" class="Symbol">=</a> <a id="1150" href="foundation-core.dependent-pair-types.html#592" class="Field">pr1</a>

<a id="is-commutative-Comm-Ring"></a><a id="1155" href="ring-theory.commutative-rings.html#1155" class="Function">is-commutative-Comm-Ring</a> <a id="1180" class="Symbol">:</a>
  <a id="1184" class="Symbol">{</a> <a id="1186" href="ring-theory.commutative-rings.html#1186" class="Bound">l</a> <a id="1188" class="Symbol">:</a> <a id="1190" href="Agda.Primitive.html#597" class="Postulate">Level</a><a id="1195" class="Symbol">}</a> <a id="1197" class="Symbol">(</a><a id="1198" href="ring-theory.commutative-rings.html#1198" class="Bound">R</a> <a id="1200" class="Symbol">:</a> <a id="1202" href="ring-theory.commutative-rings.html#991" class="Function">Comm-Ring</a> <a id="1212" href="ring-theory.commutative-rings.html#1186" class="Bound">l</a><a id="1213" class="Symbol">)</a> <a id="1215" class="Symbol">→</a> <a id="1217" href="ring-theory.commutative-rings.html#610" class="Function">is-commutative-Ring</a> <a id="1237" class="Symbol">(</a><a id="1238" href="ring-theory.commutative-rings.html#1078" class="Function">ring-Comm-Ring</a> <a id="1253" href="ring-theory.commutative-rings.html#1198" class="Bound">R</a><a id="1254" class="Symbol">)</a>
<a id="1256" href="ring-theory.commutative-rings.html#1155" class="Function">is-commutative-Comm-Ring</a> <a id="1281" class="Symbol">=</a> <a id="1283" href="foundation-core.dependent-pair-types.html#604" class="Field">pr2</a>
</pre>